examples/crypto/EtM.AE.fst
@@ -1,0 +1,54 @@
+module EtM.AE 
+
+open FStar.Seq
+open FStar.SeqProperties
+open FStar.Monotonic.Seq
+open FStar.HyperHeap
+open FStar.Monotonic.RRef
+
+
+open Platform.Bytes
+open CoreCrypto
+
+module CPA = EtM.CPA
+module MAC = EtM.MAC
+
+type log_t (r:rid) = Monotonic.Seq.log_t r (CPA.msg * CPA.cipher * MAC.tag)
+
+noeq type key = 
+  | Key:  #region:rid -> ke:CPA.key -> km:MAC.key -> log:log_t region -> key 
+  (* currently needs flag --__temp_no_proj EtM.AE *)
+
+type cipher = (CPA.cipher * MAC.tag) 
+
+let genPost parent h0 (k:key) h1 =
+    modifies Set.empty h0 h1
+  /\ extends k.region parent
+  /\ fresh_region k.region h0 h1
+  /\ m_contains k.log h1
+  /\ m_sel h1 k.log == createEmpty
+
+val keygen: parent:rid -> ST key
+  (requires (fun _ -> True))
+  (ensures  (genPost parent))
+
+
+let keygen parent =
+  let ke = CPA.gen parent in
+  let ka = MAC.gen parent in
+  let region = new_region parent in
+  let log = alloc_mref_seq region createEmpty in
+  Key #region ke ka log
+
+
+val encrypt: k:key -> EtM.Plain.plain -> cipher
+let encrypt k plain =
+  let c = CPA.encrypt k.ke plain in
+  (c, MAC.mac k.km c)
+  
+
+val decrypt: k:key -> c:cipher -> option EtM.Plain.plain
+let decrypt k (c,tag) =
+  if MAC.verify k.km c tag
+  then ( admit(); Some(CPA.decrypt k.ke c) )
+  else None
